#
#  Copyright © 2015 LiST Inc. Some Rights Reserved.
#
#  This work is licensed under the Creative Commons Attribution 4.0
#  International License. To view a copy of this license, visit
#  http://creativecommons.org/licenses/by/4.0/ or send a letter to Creative
#  Commons, 444 Castro Street, Suite 900, Mountain View, California, 94041,
#  USA.
#
#  This copyright applies only to the Juso Ontology Specification and
#  accompanying documentation in RDF or Turtle; it does not apply to data
#  formats, ontology terms, or technology. Regarding underlying technology,
#  Juso Ontology relies heavily on W3C's RDF technology, an open Web
#  standard that can be freely used by anyone.
#
#  Most of the descriptions given here are from Wikipedia or from the related
#  ontologies and vocabularies.
#

@prefix xsd: <http://www.w3.org/2001/XMLSchema#> .
@prefix rdf: <http://www.w3.org/1999/02/22-rdf-syntax-ns#> .
@prefix rdfs: <http://www.w3.org/2000/01/rdf-schema#> .
@prefix owl: <http://www.w3.org/2002/07/owl#> .
@prefix skos: <http://www.w3.org/2004/02/skos/core#> .
@prefix adms: <http://www.w3.org/ns/adms#> .
@prefix vann: <http://purl.org/vocab/vann/> .
@prefix status: <http://www.w3.org/2003/06/sw-vocab-status/ns#> .
@prefix voaf: <http://purl.org/vocommons/voaf#> .
@prefix dcam: <http://purl.org/dc/dcam/> .
@prefix dcterms: <http://purl.org/dc/terms/> .
@prefix cc: <http://creativecommons.org/ns#> .
@prefix foaf: <http://xmlns.com/foaf/0.1/> .
@prefix org: <http://www.w3.org/ns/org#> .
@prefix dbpedia: <http://dbpedia.org/ontology/> .
@prefix schema: <http://schema.org/> .
@prefix vcard: <http://www.w3.org/2006/vcard/ns#> .
@prefix ic: <http://ontology.eil.utoronto.ca/icontact.owl#> .
@prefix geo: <http://www.w3.org/2003/01/geo/wgs84_pos#> .
@prefix gsp: <http://www.opengis.net/ont/geosparql#> .
@prefix spatial: <http://geovocab.org/spatial#> .
@prefix ngeo: <http://geovocab.org/geometry#> .
@prefix gn: <http://www.geonames.org/ontology#> .
@prefix lgdo: <http://linkedgeodata.org/ontology/> .
@prefix locn: <http://www.w3.org/ns/locn#> .
@prefix juso: <http://rdfs.co/juso/> .

# Ontology ####################################################################

<http://rdfs.co/juso/0.1>
  a owl:Ontology , adms:SemanticAsset , voaf:Vocabulary , cc:Work ;
  dcterms:title "Juso Ontology"@en , "주소 온톨로지"@ko ;
  dcterms:description """
    Juso Ontology is a Web vocabulary for describing geographical addresses and
    features.
    """@en ;
  rdfs:comment """
    <div>
      The master version of this vocabulary is maintained in <a
      href="https://github.com/listinc/juso-ontology">the GitHub repository</a>
      so others can contribute edits and improvements.
    </div>
    """^^rdf:XMLLiteral ;
  rdfs:comment """
    Most of the descriptions given here are from Wikipedia or from the related
    ontologies and vocabularies.
    """@en , """
    There is an extension to this ontology with some country-specific terms for
    <a href="http://rdfs.co/juso/kr/">South Korea</a>.
    """@ko;
  vann:termGroup
    juso:CoreGroup ,
    juso:PoliticalDivisionGroup ,
    juso:AddressGroup ;
  rdfs:seeAlso <https://github.com/listinc/juso-ontology> ;
  dcterms:creator <http://jayg.me/> ;
  dcterms:publisher <http://listinc.kr/id/listinc> ;
  vann:preferredNamespaceUri "http://rdfs.co/juso/" ;
  vann:preferredNamespacePrefix "juso" ;
  dcterms:type <http://purl.org/adms/assettype/Ontology> ;
  adms:status <http://purl.org/adms/status/UnderDevelopment> ;
  dcterms:issued "2015-10-02+09:00"^^xsd:date ;
  dcterms:modified "2015-10-02+09:00"^^xsd:date ;
  dcterms:identifier "http://rdfs.co/juso/0.1" ;
  dcterms:isVersionOf <http://rdfs.co/juso/> ;
  owl:versionInfo "0.1" ;
  vann:example _:example1 ;
  dcterms:hasFormat
    <http://rdfs.co/juso/0.1/html> ,
    <http://rdfs.co/juso/0.1/ttl> ,
    <http://rdfs.co/juso/0.1/rdf> ;
  dcterms:rights
    "Copyright © 2015 LiST Inc. Some Rights Reserved." ;
  cc:license <http://creativecommons.org/licenses/by/4.0/> .

<http://rdfs.co/juso/0.1/html> dcterms:format [
  a dcterms:MediaType ;
  dcam:memberOf dcterms:IMT ;
  rdf:value "text/html" ;
  rdfs:label "HTML"@en ;
  rdfs:seeAlso <http://www.iana.org/assignments/media-types/text/html>
] .

<http://rdfs.co/juso/0.1/ttl> dcterms:format [
  a dcterms:MediaType ;
  dcam:memberOf dcterms:IMT ;
  rdf:value "text/turtle" ;
  rdfs:label "Turtle"@en ;
  rdfs:seeAlso <http://www.iana.org/assignments/media-types/text/turtle>
] .

<http://rdfs.co/juso/0.1/rdf> dcterms:format [
  a dcterms:MediaType ;
  dcam:memberOf dcterms:IMT ;
  rdf:value "application/rdf+xml" ;
  rdfs:label "RDF/XML"@en ;
  rdfs:seeAlso
    <http://www.iana.org/assignments/media-types/application/rdf+xml>
] .

<http://jayg.me/> a foaf:Person ;
  owl:sameAs <http://listinc.kr/id/member/jgkim> ;
  foaf:name "James G. Kim"@en , "김보람"@ko ;
  foaf:mbox_sha1sum "f03421e94730da58e8943d3a1d2c4c6b02898e14" ;
  foaf:homepage <http://jayg.org/> ;
  org:memberOf <http://listinc.kr/id/listinc> .

<http://listinc.kr/id/listinc> a foaf:Organization , org:Organization ;
  foaf:name "LiST Inc."@en , "주식회사 리스트"@ko ;
  foaf:mbox_sha1sum "de068365487dd2da1f2e88f1eaad0217bff79b40" ;
  foaf:homepage <http://listinc.kr/> , <http://li-st.com/> ;
  foaf:member <http://listinc.kr/id/member/jgkim> .

# Term Groups #################################################################

juso:CoreGroup a rdf:Bag ;
  rdfs:label "Core Terms"@en ;
  rdfs:comment """
    These classes and properties form the core of Juso Ontology. They describe
    fundamental characteristics of geography in relatively broad terms.
    """@en ;
  rdf:_1 juso:SpatialThing ;
  rdf:_2 juso:Feature ;
  rdf:_3 juso:Geometry ;
  rdf:_4 juso:Address ;
  rdf:_5 juso:name ;
  rdf:_6 juso:within ;
  rdf:_7 juso:endonym ;
  rdf:_8 juso:exonym ;
  rdf:_9 juso:geometry ;
  rdf:_10 juso:address ;
  rdf:_11 juso:historical_address .

juso:PoliticalDivisionGroup a rdf:Bag ;
  rdfs:label "Political Division Terms"@en ;
  rdfs:comment """
    These classes and properties are used to describe political and
    administrative divisions.
    """@en ;
  rdf:_1 juso:PoliticalDivision ;
  rdf:_2 juso:Country ;
  rdf:_3 juso:AdministrativeDivision ;
  rdf:_4 juso:FirstLevelAdministrativeDivision ;
  rdf:_5 juso:SecondLevelAdministrativeDivision ;
  rdf:_6 juso:ThirdLevelAdministrativeDivision ;
  rdf:_7 juso:FourthLevelAdministrativeDivision ;
  rdf:_8 juso:FifthLevelAdministrativeDivision ;
  rdf:_9 juso:FederatedState ;
  rdf:_10 juso:Province ;
  rdf:_11 juso:County ;
  rdf:_12 juso:Parish ;
  rdf:_13 juso:Borough ;
  rdf:_14 juso:CapitalDistrict ;
  rdf:_15 juso:City ;
  rdf:_16 juso:ConsolidatedCityCounty ;
  rdf:_17 juso:Municipality ;
  rdf:_18 juso:District ;
  rdf:_19 juso:Town ;
  rdf:_20 juso:Township ;
  rdf:_21 juso:Neighborhood ;
  rdf:_22 juso:Village ;
  rdf:_23 juso:Hamlet ;
  rdf:_24 juso:political_division ;
  rdf:_25 juso:parent .

juso:AddressGroup a rdf:Bag ;
  rdfs:label "Address Terms"@en ;
  rdfs:comment """
    These classes and properties are used to describe addresses.
    """@en ;
  rdf:_1 juso:full_address ;
  rdf:_2 juso:country ;
  rdf:_3 juso:first_level_administrative_division ;
  rdf:_4 juso:second_level_administrative_division ;
  rdf:_5 juso:third_level_administrative_division ;
  rdf:_6 juso:fourth_level_administrative_division ;
  rdf:_7 juso:fifth_level_administrative_division ;
  rdf:_8 juso:Thoroughfare ;
  rdf:_9 juso:Street ;
  rdf:_10 juso:thoroughfare ;
  rdf:_11 juso:thoroughfare_address ;
  rdf:_12 juso:locator ;
  rdf:_13 juso:locator_address ;
  rdf:_14 juso:po_box ;
  rdf:_15 juso:PostalCode ;
  rdf:_16 juso:postal_code .

# Classes #####################################################################

juso:SpatialThing a owl:Class ;
  owl:sameAs geo:SpatialThing , gsp:SpatialObject ;
  skos:prefLabel "Spatial Thing"@en ;
  skos:altLabel "Spatial Object"@en ;
  skos:definition """
    Anything that has a spatial representation, i.e. size, shape, or position.
    e.g. people, places, objects, as well as abstract areas like cubes.
    """@en ;
  rdfs:isDefinedBy <http://rdfs.co/juso/> ;
  dcterms:issued "2015-10-02+09:00"^^xsd:date ;
  dcterms:modified "2015-10-02+09:00"^^xsd:date ;
  status:term_status "testing"@en .

juso:Feature a owl:Class ;
  owl:sameAs spatial:Feature ;
  owl:equivalentClass gn:Feature ;
  rdfs:subClassOf juso:SpatialThing , gsp:Feature ;
  owl:disjointWith juso:Geometry ;
  skos:prefLabel "Geographical Feature"@en ;
  skos:altLabel "Feature"@en ;
  skos:definition """
    Geographical features are man-made or naturally-created features associated
    with a location relative to the Earth.
    """@en ;
  rdfs:seeAlso <https://en.wikipedia.org/wiki/Geographical_feature> ;
  rdfs:isDefinedBy <http://rdfs.co/juso/> ;
  dcterms:issued "2015-10-02+09:00"^^xsd:date ;
  dcterms:modified "2015-10-02+09:00"^^xsd:date ;
  status:term_status "unstable"@en .

juso:Geometry a owl:Class ;
  owl:sameAs ngeo:Geometry , gsp:Geometry , locn:Geometry ;
  rdfs:subClassOf juso:SpatialThing ;
  owl:disjointWith juso:Feature ;
  skos:prefLabel "Geometry"@en , "기하"@ko ;
  skos:definition """
    Geometry provides "the means for the quantitative description, by means of
    coordinates and mathematical functions, of the spatial characteristics of
    features, including dimension, position, size, shape, and orientation", as
    defined in ISO 19107.
    """@en ;
  rdfs:seeAlso <https://en.wikipedia.org/wiki/Geometry> ;
  rdfs:isDefinedBy <http://rdfs.co/juso/> ;
  dcterms:issued "2015-10-02+09:00"^^xsd:date ;
  dcterms:modified "2015-10-02+09:00"^^xsd:date ;
  status:term_status "unstable"@en .

juso:Address a owl:Class ;
  owl:sameAs locn:Address , ic:Address ;
  skos:prefLabel "Address"@en , "주소"@ko ;
  skos:altLabel "Geographical Address"@en , "Postal Address"@en ;
  skos:definition """
    An address is a collection of information, presented in a mostly fixed
    format, used for describing the location of a building, apartment, or other
    structure or a plot of land, generally using political boundaries and
    street names as references, along with other identifiers such as house or
    apartment numbers. Some addresses also contain special codes to aid routing
    of mail and packages, such as a ZIP code or post code.
    """@en ;
  rdfs:seeAlso <https://en.wikipedia.org/wiki/Address_(geography)> ;
  rdfs:isDefinedBy <http://rdfs.co/juso/> ;
  dcterms:issued "2015-10-02+09:00"^^xsd:date ;
  dcterms:modified "2015-10-02+09:00"^^xsd:date ;
  status:term_status "testing"@en .

juso:PoliticalDivision a owl:Class ;
  owl:equivalentClass schema:AdministrativeArea ;
  rdfs:subClassOf juso:Feature ;
  skos:prefLabel "Political Division"@en ;
  skos:definition """
    A political division is a geographic region accepted to be in the
    jurisdiction of a particular governmental entity. The particular government
    entity varies as each organizes its operations by further divisions
    (subdivisions of the state) to further its tasks and satisfy its
    responsibilities.
    """@en ;
  rdfs:seeAlso <https://en.wikipedia.org/wiki/Political_division> ;
  rdfs:isDefinedBy <http://rdfs.co/juso/> ;
  dcterms:issued "2015-10-02+09:00"^^xsd:date ;
  dcterms:modified "2015-10-02+09:00"^^xsd:date ;
  status:term_status "unstable"@en .

juso:Country a owl:Class ;
  owl:sameAs dbpedia:Country , schema:Country , lgdo:Country ;
  rdfs:subClassOf juso:PoliticalDivision ;
  skos:prefLabel "Country"@en , "나라"@ko , "国"@ja ;
  skos:altLabel "국가"@ko , "国家"@ja ;
  skos:definition """
    A country is a region that is identified as a distinct entity in political
    geography. A country may be an independent sovereign state or one that is
    occupied by another state, as a non-sovereign or formerly sovereign
    political division, or a geographic region associated with sets of
    previously independent or differently associated people with distinct
    political characteristics.
    """@en ;
  rdfs:seeAlso <https://en.wikipedia.org/wiki/Country> ;
  rdfs:isDefinedBy <http://rdfs.co/juso/> ;
  dcterms:issued "2015-10-02+09:00"^^xsd:date ;
  dcterms:modified "2015-10-02+09:00"^^xsd:date ;
  status:term_status "unstable"@en .

juso:AdministrativeDivision a owl:Class ;
  rdfs:subClassOf juso:PoliticalDivision ;
  skos:prefLabel "Administrative Division"@en ;
  skos:altLabel
    "Administrative Unit"@en ,
    "Administrative Entity"@en ,
    "Country Subdivision"@en ,
    "Geopolitical Division"@en ,
    "Subnational Entity"@en ;
  skos:definition """
    An administrative division is a portion of a country or other region
    delineated for the purpose of administration. Administrative divisions are
    each granted a certain degree of autonomy and are usually required to
    manage themselves through their own local governments.
    """@en ;
  rdfs:seeAlso
    <https://en.wikipedia.org/wiki/Administrative_division> , gn:A.ADMD ;
  rdfs:isDefinedBy <http://rdfs.co/juso/> ;
  dcterms:issued "2015-10-02+09:00"^^xsd:date ;
  dcterms:modified "2015-10-02+09:00"^^xsd:date ;
  status:term_status "unstable"@en .

juso:FirstLevelAdministrativeDivision a owl:Class ;
  rdfs:subClassOf juso:AdministrativeDivision ;
  skos:prefLabel "First-level Administrative Division"@en ;
  skos:altLabel
    "First-order Administrative Division"@en ,
    "First Administrative Level"@en ;
  skos:definition """
    A primary administrative division of a country, such as a state in the
    United States.
    """@en ;
  rdfs:seeAlso gn:A.ADM1 ;
  rdfs:isDefinedBy <http://rdfs.co/juso/> ;
  dcterms:issued "2015-10-02+09:00"^^xsd:date ;
  dcterms:modified "2015-10-02+09:00"^^xsd:date ;
  status:term_status "unstable"@en .

juso:SecondLevelAdministrativeDivision a owl:Class ;
  rdfs:subClassOf juso:AdministrativeDivision ;
  skos:prefLabel "Second-level Administrative Division"@en ;
  skos:altLabel
    "Second-order Administrative Division"@en ,
    "Second Administrative Level"@en ;
  skos:definition """
    A subdivision of a first-level administrative division.
    """@en ;
  rdfs:seeAlso gn:A.ADM2 ;
  rdfs:isDefinedBy <http://rdfs.co/juso/> ;
  dcterms:issued "2015-10-02+09:00"^^xsd:date ;
  dcterms:modified "2015-10-02+09:00"^^xsd:date ;
  status:term_status "unstable"@en .

juso:ThirdLevelAdministrativeDivision a owl:Class ;
  rdfs:subClassOf juso:AdministrativeDivision ;
  skos:prefLabel "Third-level Administrative Division"@en ;
  skos:altLabel
    "Third-order Administrative Division"@en ,
    "Third Administrative Level"@en ;
  skos:definition """
    A subdivision of a second-level administrative division.
    """@en ;
  rdfs:seeAlso gn:A.ADM3 ;
  rdfs:isDefinedBy <http://rdfs.co/juso/> ;
  dcterms:issued "2015-10-02+09:00"^^xsd:date ;
  dcterms:modified "2015-10-02+09:00"^^xsd:date ;
  status:term_status "unstable"@en .

juso:FourthLevelAdministrativeDivision a owl:Class ;
  rdfs:subClassOf juso:AdministrativeDivision ;
  skos:prefLabel "Fourth-level Administrative Division"@en ;
  skos:altLabel
    "Fourth-order Administrative Division"@en ,
    "Fourth Administrative Level"@en ;
  skos:definition """
    A subdivision of a third-level administrative division.
    """@en ;
  rdfs:seeAlso gn:A.ADM4 ;
  rdfs:isDefinedBy <http://rdfs.co/juso/> ;
  dcterms:issued "2015-10-02+09:00"^^xsd:date ;
  dcterms:modified "2015-10-02+09:00"^^xsd:date ;
  status:term_status "unstable"@en .

juso:FifthLevelAdministrativeDivision a owl:Class ;
  rdfs:subClassOf juso:AdministrativeDivision ;
  skos:prefLabel "Fifth-level Administrative Division"@en ;
  skos:altLabel
    "Fifth-order Administrative Division"@en ,
    "Fifth Administrative Level"@en ;
  skos:definition """
    A subdivision of a fourth-level administrative division.
    """@en ;
  rdfs:seeAlso gn:A.ADM5 ;
  rdfs:isDefinedBy <http://rdfs.co/juso/> ;
  dcterms:issued "2015-10-02+09:00"^^xsd:date ;
  dcterms:modified "2015-10-02+09:00"^^xsd:date ;
  status:term_status "unstable"@en .

juso:FederatedState a owl:Class ;
  rdfs:subClassOf
    juso:AdministrativeDivision ,
    dbpedia:State ,
    schema:State ,
    lgdo:State ;
  skos:prefLabel "Federated State"@en , "연방주"@ko ;
  skos:altLabel "State"@en , "주"@ko ;
  skos:definition """
    A federated state is a territorial and constitutional community forming
    part of a federal union (federation) such as the United States and
    Australia.
    """@en ;
  rdfs:seeAlso <https://en.wikipedia.org/wiki/Federated_state> ;
  rdfs:isDefinedBy <http://rdfs.co/juso/> ;
  dcterms:issued "2015-10-02+09:00"^^xsd:date ;
  dcterms:modified "2015-10-02+09:00"^^xsd:date ;
  status:term_status "unstable"@en .

juso:Province a owl:Class ;
  owl:sameAs dbpedia:Province ;
  rdfs:subClassOf juso:AdministrativeDivision , schema:State ;
  skos:prefLabel "Province"@en , "도"@ko ;
  skos:definition """
    A province is almost always an administrative division, within a country or
    state.
    """@en ;
  rdfs:seeAlso <https://en.wikipedia.org/wiki/Province> ;
  rdfs:isDefinedBy <http://rdfs.co/juso/> ;
  dcterms:issued "2015-10-02+09:00"^^xsd:date ;
  dcterms:modified "2015-10-02+09:00"^^xsd:date ;
  status:term_status "unstable"@en .

juso:County a owl:Class ;
  owl:sameAs lgdo:County ;
  rdfs:subClassOf juso:AdministrativeDivision ;
  skos:prefLabel "County"@en , "군"@ko ;
  skos:altLabel "Cnty."@en-US , "Co."@en-GB ;
  skos:definition """
    A county is a geographical region of a country used for administrative or
    other purposes, in certain modern nations.
    """@en ;
  rdfs:seeAlso <https://en.wikipedia.org/wiki/County> ;
  rdfs:isDefinedBy <http://rdfs.co/juso/> ;
  dcterms:issued "2015-10-02+09:00"^^xsd:date ;
  dcterms:modified "2015-10-02+09:00"^^xsd:date ;
  status:term_status "unstable"@en .

juso:Parish a owl:Class ;
  rdfs:subClassOf juso:AdministrativeDivision ;
  skos:prefLabel "Parish"@en ;
  skos:altLabel "Civil Parish"@en-GB ;
  skos:definition """
    A parish is an administrative division used by several countries. In parts
    of the British Isles it is known as a civil parish to distinguish it from
    the ecclesiastical parish.
    """@en ;
  rdfs:seeAlso
    <https://en.wikipedia.org/wiki/Parish_(administrative_division)> ;
  rdfs:isDefinedBy <http://rdfs.co/juso/> ;
  dcterms:issued "2015-10-02+09:00"^^xsd:date ;
  dcterms:modified "2015-10-02+09:00"^^xsd:date ;
  status:term_status "unstable"@en .

juso:CapitalDistrict a owl:Class ;
  rdfs:subClassOf juso:AdministrativeDivision ;
  skos:prefLabel "Capital District"@en ;
  skos:altLabel "Capital Territory"@en ;
  skos:definition """
    A capital district or capital territory is normally a specially designated
    administrative division where a country's seat of government is located.
    """@en ;
  rdfs:seeAlso
    <https://en.wikipedia.org/wiki/Capital_districts_and_territories> ;
  rdfs:isDefinedBy <http://rdfs.co/juso/> ;
  dcterms:issued "2015-10-02+09:00"^^xsd:date ;
  dcterms:modified "2015-10-02+09:00"^^xsd:date ;
  status:term_status "unstable"@en .

juso:City a owl:Class ;
  owl:sameAs dbpedia:City , lgdo:City ;
  rdfs:subClassOf juso:AdministrativeDivision , schema:City ;
  skos:prefLabel "City"@en , "시"@ko , "市"@ja ;
  skos:definition """
    A city is a large and permanent human settlement. Although there is no
    agreement on how a city is distinguished from a town in general English
    language meanings, many cities have a particular administrative, legal, or
    historical status based on local law.
    """@en ;
  rdfs:seeAlso <https://en.wikipedia.org/wiki/City> ;
  rdfs:isDefinedBy <http://rdfs.co/juso/> ;
  dcterms:issued "2015-10-02+09:00"^^xsd:date ;
  dcterms:modified "2015-10-02+09:00"^^xsd:date ;
  status:term_status "unstable"@en .

juso:ConsolidatedCityCounty a owl:Class ;
  rdfs:subClassOf juso:City , juso:County ;
  skos:prefLabel "Consolidated City-county"@en ;
  skos:definition """
    A consolidated city-county is a city and county that have been merged into
    one unified jurisdiction. As such it is simultaneously a city, which is a
    municipal corporation, and a county, which is an administrative division of
    a state. It has the powers and responsibilities of both types of entities.
    """@en ;
  rdfs:seeAlso <https://en.wikipedia.org/wiki/Consolidated_city-county> ;
  rdfs:isDefinedBy <http://rdfs.co/juso/> ;
  dcterms:issued "2015-10-02+09:00"^^xsd:date ;
  dcterms:modified "2015-10-02+09:00"^^xsd:date ;
  status:term_status "unstable"@en .

juso:Municipality a owl:Class ;
  owl:sameAs dbpedia:Municipality , lgdo:Municipality ;
  rdfs:subClassOf juso:AdministrativeDivision ;
  skos:prefLabel "Municipality"@en ;
  skos:definition """
    A municipality is usually an urban administrative division having corporate
    status and usually powers of self-government or jurisdiction.
    """@en ;
  rdfs:seeAlso <https://en.wikipedia.org/wiki/Municipality> ;
  rdfs:isDefinedBy <http://rdfs.co/juso/> ;
  dcterms:issued "2015-10-02+09:00"^^xsd:date ;
  dcterms:modified "2015-10-02+09:00"^^xsd:date ;
  status:term_status "unstable"@en .

juso:District a owl:Class ;
  owl:sameAs dbpedia:District ;
  rdfs:subClassOf juso:AdministrativeDivision ;
  skos:prefLabel "District"@en , "구"@ko ;
  skos:definition """
    A district is a type of administrative division that, in some countries, is
    managed by local government. Across the world, areas known as "districts"
    vary greatly in size, spanning entire regions or counties, several
    municipalities, subdivisions of municipalities, school district, or
    political district.
    """@en ;
  rdfs:seeAlso <https://en.wikipedia.org/wiki/District> ;
  rdfs:isDefinedBy <http://rdfs.co/juso/> ;
  dcterms:issued "2015-10-02+09:00"^^xsd:date ;
  dcterms:modified "2015-10-02+09:00"^^xsd:date ;
  status:term_status "unstable"@en .

juso:Town a owl:Class ;
  owl:sameAs dbpedia:Town , lgdo:Town ;
  rdfs:subClassOf juso:AdministrativeDivision ;
  skos:prefLabel "Town"@en , "읍"@ko ;
  skos:definition """
    A town is a human settlement larger than a village but smaller than a city.
    The size definition for what constitutes a "town" varies considerably in
    different parts of the world.
    """@en ;
  rdfs:seeAlso <https://en.wikipedia.org/wiki/Town> ;
  rdfs:isDefinedBy <http://rdfs.co/juso/> ;
  dcterms:issued "2015-10-02+09:00"^^xsd:date ;
  dcterms:modified "2015-10-02+09:00"^^xsd:date ;
  status:term_status "unstable"@en .

juso:Township a owl:Class ;
  rdfs:subClassOf juso:AdministrativeDivision ;
  skos:prefLabel "Township"@en , "면"@ko ;
  skos:definition """
    The word township is used to refer to different kinds of settlements in
    different countries.
    """@en ;
  rdfs:seeAlso <https://en.wikipedia.org/wiki/Township> ;
  rdfs:isDefinedBy <http://rdfs.co/juso/> ;
  dcterms:issued "2015-10-02+09:00"^^xsd:date ;
  dcterms:modified "2015-10-02+09:00"^^xsd:date ;
  status:term_status "unstable"@en .

juso:Neighborhood a owl:Class ;
  rdfs:subClassOf juso:AdministrativeDivision ;
  skos:prefLabel "Neighborhood"@en-US , "Neighbourhood"@en-GB , "동"@ko ;
  skos:definition """
    A neighborhood, or neighbourhood, is a geographically localised community
    within a larger city, town, suburb or rural area.
    """@en ;
  rdfs:seeAlso <https://en.wikipedia.org/wiki/Neighbourhood> ;
  rdfs:isDefinedBy <http://rdfs.co/juso/> ;
  dcterms:issued "2015-10-02+09:00"^^xsd:date ;
  dcterms:modified "2015-10-02+09:00"^^xsd:date ;
  status:term_status "unstable"@en .

juso:Village a owl:Class ;
  owl:sameAs dbpedia:Village , lgdo:Village ;
  rdfs:subClassOf juso:AdministrativeDivision ;
  skos:prefLabel "Village"@en , "리"@ko ;
  skos:definition """
    A village is a clustered human settlement or community, larger than a
    hamlet but smaller than a town, with a population ranging from a few
    hundred to a few thousand.
    """@en ;
  rdfs:seeAlso <https://en.wikipedia.org/wiki/Village> ;
  rdfs:isDefinedBy <http://rdfs.co/juso/> ;
  dcterms:issued "2015-10-02+09:00"^^xsd:date ;
  dcterms:modified "2015-10-02+09:00"^^xsd:date ;
  status:term_status "unstable"@en .

juso:Hamlet a owl:Class ;
  owl:sameAs lgdo:Hamlet ;
  rdfs:subClassOf juso:AdministrativeDivision ;
  skos:prefLabel "Hamlet"@en ;
  skos:definition """
    A hamlet is a type of settlement. The definition of hamlet varies by
    country. It usually refers to a small settlement, with a small population
    that is usually under 100, in a rural area, or a component of a larger
    settlement or municipality. Hamlets are typically unincorporated
    communities.
    """@en ;
  rdfs:seeAlso <https://en.wikipedia.org/wiki/Hamlet_(place)> ;
  rdfs:isDefinedBy <http://rdfs.co/juso/> ;
  dcterms:issued "2015-10-02+09:00"^^xsd:date ;
  dcterms:modified "2015-10-02+09:00"^^xsd:date ;
  status:term_status "unstable"@en .

juso:Thoroughfare a owl:Class ;
  rdfs:subClassOf juso:Feature ;
  skos:prefLabel "Thoroughfare"@en ;
  skos:definition """
    A passage or way through from one location to another, which is usually
    used a component of an address. A thoroughfare is not necessarily a road,
    it might be a waterway or some other feature.
    """@en ;
  rdfs:seeAlso <https://en.wikipedia.org/wiki/Thoroughfare> ;
  rdfs:isDefinedBy <http://rdfs.co/juso/> ;
  dcterms:issued "2015-10-02+09:00"^^xsd:date ;
  dcterms:modified "2015-10-02+09:00"^^xsd:date ;
  status:term_status "unstable"@en .

juso:Street a owl:Class ;
  rdfs:subClassOf juso:Thoroughfare ;
  skos:prefLabel "Street"@en ;
  skos:definition """
    A street is a public thoroughfare (usually paved) in a built environment.
    Practically all public streets in Western countries and the majority
    elsewhere (though not in Japan) are given a street or road name or at least
    a number to identify them and any addresses located along the streets.
    Alleys in some places do not have names.
    """@en ;
  rdfs:seeAlso <https://en.wikipedia.org/wiki/Street> , gn:R.ST ;
  rdfs:isDefinedBy <http://rdfs.co/juso/> ;
  dcterms:issued "2015-10-02+09:00"^^xsd:date ;
  dcterms:modified "2015-10-02+09:00"^^xsd:date ;
  status:term_status "unstable"@en .

juso:PostalCode a owl:Class ;
  skos:prefLabel "Postal Code"@en , "우편번호"@ko ;
  skos:altLabel
    "Postcode"@en ,
    "Post Code"@en ,
    "Eircode"@en ,
    "PIN Code"@en ,
    "ZIP Code"@en ;
  skos:definition """
    A postal code is a series of letters and/or digits, sometimes including
    spaces or punctuation, included in a postal address for the purpose of
    sorting mail.
    """@en ;
  rdfs:seeAlso <https://en.wikipedia.org/wiki/Postal_code> ;
  rdfs:isDefinedBy <http://rdfs.co/juso/> ;
  dcterms:issued "2015-10-02+09:00"^^xsd:date ;
  dcterms:modified "2015-10-02+09:00"^^xsd:date ;
  status:term_status "unstable"@en .

# Properties ##################################################################

juso:name a owl:DatatypeProperty ;
  rdfs:subPropertyOf dcterms:title , schema:name ;
  rdfs:domain juso:SpatialThing ;
  rdfs:range xsd:string ;
  skos:prefLabel "name"@en , "이름"@ko ;
  skos:definition """
    This property indicates the name of the spatial thing.
    """@en ;
  rdfs:isDefinedBy <http://rdfs.co/juso/> ;
  dcterms:issued "2015-10-02+09:00"^^xsd:date ;
  dcterms:modified "2015-10-02+09:00"^^xsd:date ;
  status:term_status "testing"@en .

juso:within a owl:TransitiveProperty ;
  owl:sameAs gsp:sfWithin , spatial:P ;
  owl:inverseOf gsp:sfContains , spatial:Pi ;
  rdfs:subPropertyOf geo:location , locn:location ;
  rdfs:domain juso:SpatialThing ;
  rdfs:range juso:SpatialThing ;
  skos:prefLabel "within"@en ;
  skos:definition """
    A spatial thing that contains the current one within the borders of its own
    region.
    """@en ;
  rdfs:isDefinedBy <http://rdfs.co/juso/> ;
  dcterms:issued "2015-10-02+09:00"^^xsd:date ;
  dcterms:modified "2015-10-02+09:00"^^xsd:date ;
  status:term_status "testing"@en .

juso:endonym a owl:DatatypeProperty ;
  rdfs:subPropertyOf juso:name , gn:officialName , skos:prefLabel ;
  rdfs:domain juso:Feature ;
  rdfs:range xsd:string ;
  skos:prefLabel "endonym"@en ;
  skos:definition """
    The endonym is a name given by members of a particular ethnolinguistic
    group to its homeland or a specific place within it.
    """@en ;
  rdfs:seeAlso <https://en.wikipedia.org/wiki/Exonym_and_endonym> ;
  rdfs:isDefinedBy <http://rdfs.co/juso/> ;
  dcterms:issued "2015-10-02+09:00"^^xsd:date ;
  dcterms:modified "2015-10-02+09:00"^^xsd:date ;
  status:term_status "unstable"@en .

juso:exonym a owl:DatatypeProperty ;
  rdfs:subPropertyOf juso:name , gn:alternateName , skos:altLabel ;
  rdfs:domain juso:Feature ;
  rdfs:range xsd:string ;
  skos:prefLabel "exonym"@en ;
  skos:definition """
    The exonym is an external name for a geographical place: a common name used
    only outside the place in question, usually for historical reasons.
    """@en ;
  rdfs:seeAlso <https://en.wikipedia.org/wiki/Exonym_and_endonym> ;
  rdfs:isDefinedBy <http://rdfs.co/juso/> ;
  dcterms:issued "2015-10-02+09:00"^^xsd:date ;
  dcterms:modified "2015-10-02+09:00"^^xsd:date ;
  status:term_status "unstable"@en .

juso:geometry a owl:ObjectProperty ;
  rdfs:subPropertyOf ngeo:geometry , locn:geometry ;
  rdfs:domain juso:Feature ;
  rdfs:range juso:Geometry ;
  skos:prefLabel "geometry"@en ;
  skos:definition """
    This property associates any feature with the corresponding geometry.
    """@en ;
  rdfs:isDefinedBy <http://rdfs.co/juso/> ;
  dcterms:issued "2015-10-02+09:00"^^xsd:date ;
  dcterms:modified "2015-10-02+09:00"^^xsd:date ;
  status:term_status "unstable"@en .

juso:address a owl:ObjectProperty ;
  rdfs:subPropertyOf ic:address , locn:address ;
  rdfs:domain juso:SpatialThing ;
  rdfs:range juso:Address ;
  skos:prefLabel "address"@en ;
  skos:definition """
    This property associates anything with its address.
    """@en ;
  rdfs:isDefinedBy <http://rdfs.co/juso/> ;
  dcterms:issued "2015-10-02+09:00"^^xsd:date ;
  dcterms:modified "2015-10-02+09:00"^^xsd:date ;
  status:term_status "unstable"@en .

juso:historical_address a owl:ObjectProperty ;
  rdfs:domain juso:SpatialThing ;
  rdfs:range juso:Address ;
  skos:prefLabel "historical address"@en ;
  skos:definition """
    This property associates anything with one of its historical address.
    """@en ;
  rdfs:isDefinedBy <http://rdfs.co/juso/> ;
  dcterms:issued "2015-10-02+09:00"^^xsd:date ;
  dcterms:modified "2015-10-02+09:00"^^xsd:date ;
  status:term_status "unstable"@en .

juso:political_division a owl:TransitiveProperty ;
  rdfs:domain juso:Feature ;
  rdfs:range juso:PoliticalDivision ;
  skos:prefLabel "political division"@en ;
  skos:definition """
    A politial or administrative division that contain the current feature.
    """@en ;
  rdfs:isDefinedBy <http://rdfs.co/juso/> ;
  dcterms:issued "2015-10-02+09:00"^^xsd:date ;
  dcterms:modified "2015-10-02+09:00"^^xsd:date ;
  status:term_status "unstable"@en .

juso:parent a owl:ObjectProperty ;
  rdfs:subPropertyOf juso:political_division , gn:parentFeature ;
  rdfs:domain juso:Feature ;
  rdfs:range juso:PoliticalDivision ;
  skos:prefLabel "parent politial division"@en ;
  skos:definition """
    A politial or administrative division that is a direct parent of the
    current feature.
    """@en ;
  rdfs:isDefinedBy <http://rdfs.co/juso/> ;
  dcterms:issued "2015-10-02+09:00"^^xsd:date ;
  dcterms:modified "2015-10-02+09:00"^^xsd:date ;
  status:term_status "unstable"@en .

juso:full_address a owl:DatatypeProperty ;
  owl:sameAs locn:fullAddress ;
  rdfs:domain juso:Address ;
  rdfs:range xsd:string ;
  skos:prefLabel "full address"@en ;
  skos:definition """
    The complete address written as a string, with or without formatting.
    """@en ;
  rdfs:isDefinedBy <http://rdfs.co/juso/> ;
  dcterms:issued "2015-10-02+09:00"^^xsd:date ;
  dcterms:modified "2015-10-02+09:00"^^xsd:date ;
  status:term_status "testing"@en .

juso:country a owl:ObjectProperty ;
  owl:sameAs ic:hasCountry ;
  rdfs:domain juso:Address ;
  rdfs:range juso:Country ;
  skos:prefLabel "country"@en ;
  skos:definition """
    The uppermost politial division for the address, almost always a country.
    """@en ;
  rdfs:isDefinedBy <http://rdfs.co/juso/> ;
  dcterms:issued "2015-10-02+09:00"^^xsd:date ;
  dcterms:modified "2015-10-02+09:00"^^xsd:date ;
  status:term_status "unstable"@en .

juso:first_level_administrative_division a owl:ObjectProperty ;
  rdfs:domain juso:Address ;
  rdfs:range juso:FirstLevelAdministrativeDivision ;
  skos:prefLabel "first-level administrative division"@en ;
  skos:definition """
    The first-level administrative division (region) of the address, usually a
    county, state or other such area that typically encompasses several
    localities.
    """@en ;
  rdfs:isDefinedBy <http://rdfs.co/juso/> ;
  dcterms:issued "2015-10-02+09:00"^^xsd:date ;
  dcterms:modified "2015-10-02+09:00"^^xsd:date ;
  status:term_status "unstable"@en .

juso:second_level_administrative_division a owl:ObjectProperty ;
  rdfs:domain juso:Address ;
  rdfs:range juso:SecondLevelAdministrativeDivision ;
  skos:prefLabel "second-level administrative division"@en ;
  skos:definition """
    The second-level administrative division (locality) of the address, usually
    a city.
    """@en ;
  rdfs:isDefinedBy <http://rdfs.co/juso/> ;
  dcterms:issued "2015-10-02+09:00"^^xsd:date ;
  dcterms:modified "2015-10-02+09:00"^^xsd:date ;
  status:term_status "unstable"@en .

juso:third_level_administrative_division a owl:ObjectProperty ;
  rdfs:domain juso:Address ;
  rdfs:range juso:ThirdLevelAdministrativeDivision ;
  skos:prefLabel "third-level administrative division"@en ;
  skos:definition """
    The third-level administrative division of the address, if any.
    """@en ;
  rdfs:isDefinedBy <http://rdfs.co/juso/> ;
  dcterms:issued "2015-10-02+09:00"^^xsd:date ;
  dcterms:modified "2015-10-02+09:00"^^xsd:date ;
  status:term_status "unstable"@en .

juso:fourth_level_administrative_division a owl:ObjectProperty ;
  rdfs:domain juso:Address ;
  rdfs:range juso:FourthLevelAdministrativeDivision ;
  skos:prefLabel "fourth-level administrative division"@en ;
  skos:definition """
    The fourth-level administrative division of the address, if any.
    """@en ;
  rdfs:isDefinedBy <http://rdfs.co/juso/> ;
  dcterms:issued "2015-10-02+09:00"^^xsd:date ;
  dcterms:modified "2015-10-02+09:00"^^xsd:date ;
  status:term_status "unstable"@en .

juso:fifth_level_administrative_division a owl:ObjectProperty ;
  rdfs:domain juso:Address ;
  rdfs:range juso:FifthLevelAdministrativeDivision ;
  skos:prefLabel "fifth-level administrative division"@en ;
  skos:definition """
    The fifth-level administrative division of the address, if any.
    """@en ;
  rdfs:isDefinedBy <http://rdfs.co/juso/> ;
  dcterms:issued "2015-10-02+09:00"^^xsd:date ;
  dcterms:modified "2015-10-02+09:00"^^xsd:date ;
  status:term_status "unstable"@en .

juso:thoroughfare a owl:ObjectProperty ;
  rdfs:domain juso:Address ;
  rdfs:range juso:Thoroughfare ;
  skos:prefLabel "thoroughfare"@en ;
  skos:definition """
    An address component that represents the name of a passage or way through
    from one location to another. A thoroughfare is not necessarily a road, it
    might be a waterway or some other feature.
    """@en ;
  rdfs:isDefinedBy <http://rdfs.co/juso/> ;
  dcterms:issued "2015-10-02+09:00"^^xsd:date ;
  dcterms:modified "2015-10-02+09:00"^^xsd:date ;
  status:term_status "unstable"@en .

juso:thoroughfare_address a owl:DatatypeProperty ;
  rdfs:domain juso:Address ;
  rdfs:range xsd:string ;
  skos:prefLabel "thoroughfare address"@en ;
  skos:definition """
    This property is used to describe a unique number given to each building
    (residential or not) or vacant lot with a mailbox in a street or other
    thoroughfares.
    """@en ;
  rdfs:seeAlso <https://en.wikipedia.org/wiki/House_numbering> ;
  rdfs:isDefinedBy <http://rdfs.co/juso/> ;
  dcterms:issued "2015-10-02+09:00"^^xsd:date ;
  dcterms:modified "2015-10-02+09:00"^^xsd:date ;
  status:term_status "unstable"@en .

juso:locator a owl:ObjectProperty ;
  rdfs:domain juso:Address ;
  rdfs:range juso:Feature ;
  skos:prefLabel "locator"@en ;
  skos:definition """
    The real world entity identified by the address. The locator could be the
    property or complex, of the building or part of the building, of it could
    be a room inside a building.
    """@en ;
  rdfs:isDefinedBy <http://rdfs.co/juso/> ;
  dcterms:issued "2015-10-02+09:00"^^xsd:date ;
  dcterms:modified "2015-10-02+09:00"^^xsd:date ;
  status:term_status "unstable"@en .

juso:locator_address a owl:DatatypeProperty ;
  rdfs:domain juso:Address ;
  rdfs:range xsd:string ;
  skos:prefLabel "locator address"@en ;
  skos:definition """
    This property is used to describe a number or a sequence of characters that
    uniquely identifies the exact locator within the relevant scope(s), that is
    described by juso:locator.
    """@en ;
  rdfs:isDefinedBy <http://rdfs.co/juso/> ;
  dcterms:issued "2015-10-02+09:00"^^xsd:date ;
  dcterms:modified "2015-10-02+09:00"^^xsd:date ;
  status:term_status "unstable"@en .

juso:post_office_box a owl:DatatypeProperty ;
  owl:sameAs locn:poBox , schema:postOfficeBoxNumber ;
  rdfs:domain juso:Address ;
  rdfs:range xsd:string ;
  skos:prefLabel "post office box"@en ;
  skos:definition """
    This property describes the post office box number for PO box addresses.
    A post-office box or post office box (commonly referred to as a PO box or a
    postal box) is a uniquely addressable lockable box located on the premises
    of a post office station.
    """@en ;
  rdfs:isDefinedBy <http://rdfs.co/juso/> ;
  dcterms:issued "2015-10-02+09:00"^^xsd:date ;
  dcterms:modified "2015-10-02+09:00"^^xsd:date ;
  status:term_status "unstable"@en .

juso:postal_code a owl:DatatypeProperty ;
  rdfs:domain juso:Address ;
  rdfs:range juso:PostalCode ;
  skos:prefLabel "postal code"@en ;
  skos:definition """
    This property associates any address with its postal code.
    """@en ;
  rdfs:isDefinedBy <http://rdfs.co/juso/> ;
  dcterms:issued "2015-10-02+09:00"^^xsd:date ;
  dcterms:modified "2015-10-02+09:00"^^xsd:date ;
  status:term_status "unstable"@en .

# Relations with other ontologies and vocabularies ############################

dcterms:Location rdfs:subClassOf juso:SpatialThing .
schema:Place rdfs:subClassOf juso:SpatialThing .
lgdo:Place rdfs:subClassOf juso:SpatialThing .
geo:Point rdfs:subClassOf juso:Geometry .
schema:GeoCoordinates rdfs:subClassOf juso:Geometry .
schema:GeoShape rdfs:subClassOf juso:Geometry .
schema:PostalAddress rdfs:subClassOf juso:Address .
vcard:Address rdfs:subClassOf juso:Address .
schema:address rdfs:subPropertyOf juso:address .
schema:containedIn rdfs:subPropertyOf juso:within .
schema:geo rdfs:subPropertyOf juso:geometry .
gsp:hasGeometry rdfs:subPropertyOf juso:geometry .
ic:hasState rdfs:subPropertyOf juso:first_level_administrative_division .
ic:hasStreetNumber rdfs:subPropertyOf juso:thoroughfare_address .
ic:hasPostalCode owl:propertyChainAxiom ( juso:postal_code rdf:value ) .
locn:postCode owl:propertyChainAxiom ( juso:postal_code rdf:value ) .
schema:postalCode owl:propertyChainAxiom ( juso:postal_code rdf:value ) .
vcard:postal-code owl:propertyChainAxiom ( juso:postal_code rdf:value ) .

# Example #####################################################################

_:example1 rdfs:label "LiST Inc."@en ;
  rdfs:comment '''
    <pre><code>_:YangyongBldg a juso:Feature ;
  juso:name "Yangyong Building"@en , "양용빌딩"@ko ;
  juso:geometry &lt;http://geohash.org/wydjrzg6ece9&gt; .

_:LiSTInc a juso:SpatialThing , foaf:Organization ;
  juso:name "LiST Inc."@en , "주식회사 리스트"@ko ;
  juso:within _:YangyongBldg ;
  juso:historical_address [
    a juso:Address ;
    juso:full_address
      "대한민국 서울특별시 영등포구 당산동 121-17 양용빌딩 9층 150-040"@ko ,
      "9th Floor, Yangyong Building, 121-17, Dangsan-dong, Yeongdeungpo-gu, Seoul, 150-040, South Korea"@en ;
    juso:country &lt;http://sws.geonames.org/1835841/&gt; ;
    juso:first_level_administrative_division &lt;http://sws.geonames.org/1835847/&gt; ;
    juso:second_level_administrative_division &lt;http://sws.geonames.org/1832536/&gt; ;
    juso:third_level_administrative_division &lt;http://sws.geonames.org/8692617/&gt; ;
    juso:locator _:YangyongBldg ;
    juso:locator_address "9층"@ko , "9th Floor"@en ;
    juso:postal_code [
      a juso:PostalCode ;
      rdf:value "150-040"
    ]
  ] ;
  juso:address [
    a juso:Address ;
    juso:full_address
      "대한민국 서울특별시 영등포구 버드나루로19길 3 (당산동) 양용빌딩 9층 07229"@ko ,
      "9th Floor, Yangyong Building, 3, Beodeunaru-ro 19-gil, Yeongdeungpo-gu, Seoul, 07229, South Korea"@en ;
    juso:country &lt;http://sws.geonames.org/1835841/&gt; ;
    juso:first_level_administrative_division &lt;http://sws.geonames.org/1835847/&gt; ;
    juso:second_level_administrative_division &lt;http://sws.geonames.org/1832536/&gt; ;
    juso:third_level_administrative_division &lt;http://sws.geonames.org/8692617/&gt; ;
    juso:thoroughfare [
      a juso:Street ;
      juso:name "Beodeunaru-ro 19-gil"@en , "버드나루로19길"@ko ;
      juso:parent &lt;http://sws.geonames.org/8692617/&gt;
    ] ;
    juso:thoroughfare_address "3" ;
    juso:locator _:YangyongBldg ;
    juso:locator_address "9층"@ko , "9th Floor"@en ;
    juso:postal_code [
      a juso:PostalCode ;
      rdf:value "07229"
    ]
  ] .</code></pre>
    '''^^rdf:XMLLiteral .
